\input{en/m2-ex-01/ex-jun-2015}

\begin{comparchsol}
\end{comparchsol}

\[
S = \frac{1}{\left(1 - F \right) + \displaystyle \frac{F}{n} }
\]

\[
S \times \left( (1-F) + \frac{F}{n} \right) = 1
\]

\[
S - S \times F + \frac{S \times F}{n} = 1
\]

\[
n \times S - n \times S \times F + S \times F = n
\]

\[
n \times S - n = n \times S \times F - S \times F
\]

\[
S \times F \times \left( n - 1 \right) = n \times \left( S - 1 \right)
\]

\[
F = \frac{n \times (S-1)}{S \times(n-1)}
\]

For the case of $S = 10$

\[
F = \frac{n \times (10-1)}{10 \times (n-1)} = 
\frac{9 \times n}{10 \times n - 10}
\]

As $F$ must be less or equal than $1$:

\[
F \leq 1
\]

\[
\frac{9 \times n}{10 \times n -10} \leq 1
\]

\[
9 \times n \leq 10 \times n-10
\]

\[
n \geq 10
\]


